src/basic/ThreadBoundedExecution.v
@@ -4,13 +4,12 @@ From imm Require Import Execution Events.
 Require Import Lia.
 
 
-(* TODO: move to separate file *)
 Definition threads_bound (G: execution) (b: thread_id) :=
   forall e (Ge: acts_set G e), BinPos.Pos.lt (tid e) b.
 
 Lemma BinPos_lt_fin b:
   set_finite (fun t => BinPos.Pos.lt t b). 
-Proof.
+Proof using.
   exists (map BinPos.Pos.of_nat (List.seq 0 (BinPos.Pos.to_nat b))).
   ins. apply Pnat.Pos2Nat.inj_lt in IN. 
   apply in_map_iff. eexists. splits.
