src/imm/SubExecution.v
@@ -543,7 +543,7 @@ Qed.
 
 Lemma events_separation G:
   acts_set G ≡₁ ⋃₁ t, acts_set (restrict G (Tid_ t)).
-Proof.
+Proof using.
   unfold restrict. simpl.
   rewrite set_bunion_inter_compat_r, set_interC, <- set_bunion_inter_compat_l.
   apply set_bunion_separation. 
@@ -551,28 +551,22 @@ Qed.
 
 Lemma fin_exec_bounded_threads G b
       (TB: threads_bound G b)
-      (FIN_B: forall t (NI: t <> tid_init) (LTB: BinPos.Pos.lt t b),
-          fin_exec (restrict G (Tid_ t))):
+      (FIN_B: forall t (LTB: BinPos.Pos.lt t b), fin_exec (restrict G (Tid_ t))):
   fin_exec G. 
-Proof.
+Proof using.
   red. rewrite events_separation, <- set_bunion_minus_compat_r.
   rewrite set_full_split with (S := fun t => BinPos.Pos.lt t b).
   rewrite set_bunion_union_l. apply set_finite_union. split.
   2: { exists nil. unfold restrict. simpl. unfolder. ins. desc.
        red in TB. apply TB in IN2. congruence. }
-  apply set_finite_bunion; [by apply BinPos_lt_fin| ].
-  intros t LT.
-  destruct (classic (t = tid_init)) as [-> | NI]. 
-  2: { by apply FIN_B. }
-  exists nil. unfold restrict. simpl. unfolder. ins. by desc. 
+  apply set_finite_bunion; [by apply BinPos_lt_fin| done].
 Qed.
 
 Lemma restrict_fair G (S: actid -> Prop) (FAIR: mem_fair G):
   mem_fair (restrict G S).
-Proof.
+Proof using.
   unfold restrict, mem_fair, fr. simpl. destruct FAIR as [FSco FSfr].
   split.
   - eapply fsupp_mori; [| by apply FSco]. red. basic_solver.
   - eapply fsupp_mori; [| by apply FSfr]. red. unfold fr. basic_solver.
 Qed.
-
