src/lib/AuxRel2.v
@@ -110,12 +110,12 @@ Proof using. basic_solver. Qed.
 
 Lemma set_full_split {A: Type} (S: A -> Prop):
   set_full ≡₁ S ∪₁ set_compl S.
-Proof.
+Proof using.
   split; [| basic_solver]. red. ins. destruct (classic (S x)); basic_solver.
 Qed.
 
 Lemma set_bunion_separation {A B: Type} (S: A -> Prop) (fab: A -> B):
   S ≡₁ ⋃₁ b, S ∩₁ (fun a => fab a = b).
-Proof. basic_solver. Qed.       
+Proof using. basic_solver. Qed.       
 
 
